src/Codegen/Export/Voblint_Codegen.thy
@@ -42,6 +42,7 @@ export_code
   full_state_dot_auto full_state_graph_snapshot_auto
   entry_state_report_dot_auto entry_state_report_graph_snapshot_auto
   entry_state_full_state_dot_auto entry_state_full_state_graph_snapshot_auto
+  entry_state_ctx_dot_auto entry_state_ctx_graph_snapshot_auto
   exp_vnames_list string_of_abstract_value
   is_bottom_abstract_value program_vars
   mk_program proc_decl_of declared_global_vars pretty_string_of_program
